transition: use accessor functions instead of pattern matching as tactics do not normalise under matches

src/Pipit.System.ExpX.fst
@@ -18,13 +18,29 @@ let rec state_of_exp (e: exp): Type =
   | XThen e1 e2 -> bool * state_of_exp e2
   | XMu e1 -> state_of_exp e1
 
+type map2_oracle (value1 value2 oracle1 oracle2: Type) = {
+     m2_r1: value1;
+     m2_r2: value2;
+     m2_o1: oracle1;
+     m2_o2: oracle2;
+  }
+
+type then_oracle (state1 value2 oracle1 oracle2: Type) = {
+     then_s1:  state1;
+     then_s1': state1;
+     then_r2: value2;
+     then_o1: oracle1;
+     then_o2: oracle2;
+  }
+
+
 let rec oracle_of_exp (e: exp): Type =
   match e with
   | XVal v -> unit
   | XVar x -> unit
-  | XPrim2 p e1 e2 -> value * value * oracle_of_exp e1 * oracle_of_exp e2
+  | XPrim2 p e1 e2 -> map2_oracle value value (oracle_of_exp e1) (oracle_of_exp e2)
   | XPre e1 -> oracle_of_exp e1
-  | XThen e1 e2 -> state_of_exp e1 * state_of_exp e1 * value * oracle_of_exp e1 * oracle_of_exp e2
+  | XThen e1 e2 -> then_oracle (state_of_exp e1) value (oracle_of_exp e1) (oracle_of_exp e2)
   | XMu e1 -> oracle_of_exp e1
 
 (* An system with "oracles", which let us draw out the quantifiers to the top level *)
@@ -35,44 +51,48 @@ let xsystem (e: exp) (vars: nat { wf e vars }) = osystem (C.row vars) (oracle_of
 
 let osystem_input (#input #oracle: Type): osystem input oracle unit input =
   { init = (fun s -> True);
-    step = (fun (i, o) s s' r -> r == i) }
+    step = (fun io s s' r -> r == (fst io)) }
 
 let osystem_index (vars: nat) (x: nat { x < vars }):
        osystem (C.row vars) unit unit value =
   { init = (fun _ -> True);
-    step = (fun (i, o) s s' r ->
-      r == C.row_index i x)
+    step = (fun io s s' r ->
+      r == C.row_index (fst io) x)
   }
 
 let osystem_map2 (#input #oracle1 #oracle2 #state1 #state2 #value1 #value2 #result: Type) (f: value1 -> value2 -> result)
   (t1: osystem input oracle1 state1 value1)
   (t2: osystem input oracle2 state2 value2):
-       osystem input (value1 * value2 * oracle1 * oracle2) (state1 * state2) result =
+       osystem input (map2_oracle value1 value2 oracle1 oracle2) (state1 * state2) result =
    {
-    init = (fun (s1, s2) -> t1.init s1 /\ t2.init s2);
-    step = (fun (i, (r1, r2, o1, o2)) (s1, s2) (s1', s2') r ->
-               t1.step (i, o1) s1 s1' r1 /\
-               t2.step (i, o2) s2 s2' r2 /\
-               r == f r1 r2)
+    init = (fun s -> t1.init (fst s) /\ t2.init (snd s));
+    step = (fun io s s' r ->
+               let i = fst io in
+               let o = snd io in
+               t1.step (i, o.m2_o1) (fst s) (fst s') o.m2_r1 /\
+               t2.step (i, o.m2_o2) (snd s) (snd s') o.m2_r2 /\
+               r == f o.m2_r1 o.m2_r2)
   }
 
 let osystem_pre (#input #oracle1 #state1 #v: Type) (init: v)
   (t1: osystem input oracle1 state1 v):
        osystem input oracle1 (state1 * v) v =
-  { init = (fun (s1, v) -> t1.init s1 /\ v == init);
-    step = (fun i (s1, v) (s1', v') r ->
-      t1.step i s1 s1' v' /\ r == v)
+  { init = (fun s -> t1.init (fst s) /\ (snd s) == init);
+    step = (fun i s s' r ->
+      t1.step i (fst s) (fst s') (snd s') /\ r == (snd s))
   }
 
 let osystem_then (#input #oracle1 #oracle2 #state1 #state2 #v: Type)
   (t1: osystem input oracle1 state1 v)
   (t2: osystem input oracle2 state2 v):
-       osystem input (state1 * state1 * v * oracle1 * oracle2) (bool * state2) v =
-  { init = (fun (init,s2) -> init = true /\ t2.init s2);
-    step = (fun (i, (s1, s1', r', o1, o2)) (init, s2) (init', s2') r ->
-     if init
-     then t1.init s1 /\ t1.step (i, o1) s1 s1' r /\ t2.step (i, o2) s2 s2' r'
-     else init = false /\ t2.step (i, o2) s2 s2' r)
+       osystem input (then_oracle state1 v oracle1 oracle2) (bool * state2) v =
+  { init = (fun s -> (fst s) = true /\ t2.init (snd s));
+    step = (fun io s s' r ->
+     let i = fst io in
+     let o = snd io in
+     if (fst s)
+     then t1.init o.then_s1 /\ t1.step (i, o.then_o1) o.then_s1 o.then_s1' r /\ t2.step (i, o.then_o2) (snd s) (snd s') o.then_r2
+     else fst s = false /\ t2.step (i, o.then_o2) (snd s) (snd s') r)
   }
 
 let osystem_mu (#input #input' #oracle #state1 #v: Type)
@@ -80,7 +100,7 @@ let osystem_mu (#input #input' #oracle #state1 #v: Type)
   (t1: osystem input' oracle state1 v):
        osystem input  oracle state1 v =
   { init = t1.init;
-    step = (fun (i, o) s s' r -> t1.step (extend i r, o) s s' r)
+    step = (fun io s s' r -> t1.step (extend (fst io) r, snd io) s s' r)
   }
 
 irreducible let unfold_attr = ()
@@ -101,24 +121,6 @@ let rec osystem_of_exp (e: exp) (vars: nat { wf e vars }):
     let t = osystem_of_exp e1 (vars + 1) in
     osystem_mu #(C.row vars) #(C.row (vars + 1)) (fun i v -> C.row_append (C.row1 v) i) t
 
-// let rec osystem_of_exp_init (e: exp) (vars: nat { wf e vars }) (s: state_of_exp e): prop =
-//   match e with
-//   | XVal v -> True
-//   | XVar x -> True
-//   | XPrim2 p e1 e2 ->
-//     let ss = s <: state_of_exp e1 * state_of_exp e2 in
-//     osystem_of_exp_init e1 vars (fst ss) /\
-//     osystem_of_exp_init e2 vars (snd ss)
-//   | XPre e1 ->
-//     let ss = s <: state_of_exp e1 * value in
-//     osystem_of_exp_init e1 vars (fst ss) /\ (snd ss) = xpre_init
-//   | XThen e1 e2 ->
-//     osystem_then (osystem_of_exp e1 vars) (osystem_of_exp e2 vars)
-//   | XMu e1 ->
-//     let t = osystem_of_exp e1 (vars + 1) in
-//     osystem_mu #(C.row vars) #(C.row (vars + 1)) (fun i v -> C.row_append (C.row1 v) i) t
-
-
 module Ck = Pipit.Check.Example
 module T = FStar.Tactics
 
@@ -126,26 +128,101 @@ open Pipit.System.Ind
 
 
 
-let wf_ (): wf_: nat { wf (Ck.example0_ok Ck.x0) wf_ } = 1
 let example0_t = osystem_of_exp (Ck.example0_ok Ck.x0) 1
 
 let example0_ok_base (): Lemma (ensures base_case' example0_t) =
 
   assert (base_case' example0_t) by (
-    T.compute ();
+    // T.compute ();
+    // T.simpl ();
+    // let _ = T.forall_intro_as "x" in
     // let _ = T.forall_intros () in
     T.norm [delta_attr [`%unfold_attr]];
-    T.whnf ();
-    T.unfold_def (`osystem_of_exp);
+    // T.whnf ();
+    // T.unfold_def (`osystem_of_exp);
     // T.l_revert ();
     // T.revert ();
     // T.implies_intro ();
     // T.forall_intro ();
-    T.dump "wbase_case"
+    T.compute ();
+    T.dump "base_case"
   );
 
-  admit ()
+  ()
 
 let example0_ok_step (): Lemma (ensures step_case' example0_t) =
-  assert (step_case' example0_t) by (T.compute (); T.dump "step_case");
+  assert (step_case' example0_t) by (
+    // T.unfold_def (`example0_t);
+    // T.norm [delta_attr [`%osystem_of_exp; `%wf]];
+    // T.unfold_def (`osystem_of_exp);
+    // let _ = T.forall_intros () in
+    T.compute ();
+    T.dump "step_case");
+  ()
+
+let example1_t = osystem_of_exp (Ck.example1_bad Ck.x0) 1
+
+let example1_nok_base (): Lemma (ensures base_case' example1_t) =
+  assert (base_case' example1_t) by (T.compute ());
+  ()
+
+// this is not true, so we can't prove it
+[@@expect_failure]
+let example1_nok_step (): Lemma (ensures step_case' example1_t) =
+  assert (step_case' example1_t) by (T.compute ());
+  ()
+
+
+// always a => always (always a)
+let example_GA_GGA =
+  osystem_of_exp (
+    let open Ck in
+    let a = x0 in
+    sofar a => sofar (sofar a))
+    1
+
+let example_GA_GGA_ok (): unit =
+  assert (base_case' example_GA_GGA) by (T.compute ());
+  assert (step_case' example_GA_GGA) by (T.compute ());
+  ()
+
+// sometimes a => not (always (not a))
+let example_F_def =
+  osystem_of_exp (
+    let open Ck in
+    let a = x0 in
+    once a => Ck.not (sofar (Ck.not a)))
+    1
+
+let example_F_def_ok (): unit =
+  assert (base_case' example_F_def) by (T.compute ());
+  assert (step_case' example_F_def) by (T.compute ());
+  ()
+
+// always a /\ always (a => b) => always b
+let example_GA_GAB__GB =
+  osystem_of_exp (
+    let open Ck in
+    let a = x0 in
+    let b = x1 in
+    (sofar a /\ sofar (a => b)) => sofar b)
+    2
+
+let example_GA_GAB_GB_ok (): unit =
+  assert (base_case' example_GA_GAB__GB) by (T.compute (); T.dump "base GA_GAB_GB");
+  assert (step_case' example_GA_GAB__GB) by (T.compute (); T.dump "step GA_GAB_GB");
+  ()
+
+let example_FA_GAB__FB =
+  osystem_of_exp (
+    let open Ck in
+    let a = x0 in
+    let b = x1 in
+    (sofar (a => b)) => (once a => once b))
+    2
+
+// this seems like it should be true. why can't prove?
+let example_GA_GAB_FB_ok (): unit =
+  // assert (base_case' example_FA_GAB__FB) by (T.compute (); T.dump "base GA_FAB_FB");
+  assert (step_case' example_FA_GAB__FB) by (T.compute (); T.dump "step GA_GAB_FB");
   ()
